[Dafny] Add old-expressions
It has been added to the AST and the proofs have been fixed. However, it is not
yet supported by the frontend.

compiler/dafny/dafny_freshenScript.sml
@@ -20,130 +20,132 @@ Definition add_fresh_def:
 End
 
 Definition freshen_exp_def:
-  freshen_exp m cnt (Lit l) = (cnt, Lit l) ∧
-  freshen_exp m cnt (Var old) = (cnt, Var (lookup m old)) ∧
-  freshen_exp m cnt (If tst thn els) =
+  freshen_exp m m_old cnt (Lit l) = (cnt, Lit l) ∧
+  freshen_exp m m_old cnt (Var old) = (cnt, Var (lookup m old)) ∧
+  freshen_exp m m_old cnt (If tst thn els) =
     (let
-       (cnt, tst) = freshen_exp m cnt tst;
-       (cnt, thn) = freshen_exp m cnt thn;
-       (cnt, els) = freshen_exp m cnt els
+       (cnt, tst) = freshen_exp m m_old cnt tst;
+       (cnt, thn) = freshen_exp m m_old cnt thn;
+       (cnt, els) = freshen_exp m m_old cnt els
      in
        (cnt, If tst thn els)) ∧
-  freshen_exp m cnt (UnOp uop e) =
-    (let (cnt, e) = freshen_exp m cnt e in
+  freshen_exp m m_old cnt (UnOp uop e) =
+    (let (cnt, e) = freshen_exp m m_old cnt e in
        (cnt, UnOp uop e)) ∧
-  freshen_exp m cnt (BinOp bop e₁ e₂) =
-    (let (cnt, e₁) = freshen_exp m cnt e₁ in
-     let (cnt, e₂) = freshen_exp m cnt e₂ in
+  freshen_exp m m_old cnt (BinOp bop e₁ e₂) =
+    (let (cnt, e₁) = freshen_exp m m_old cnt e₁ in
+     let (cnt, e₂) = freshen_exp m m_old cnt e₂ in
        (cnt, BinOp bop e₁ e₂)) ∧
-  freshen_exp m cnt (ArrLen arr) =
+  freshen_exp m m_old cnt (ArrLen arr) =
     (let
-       (cnt, arr) = freshen_exp m cnt arr
+       (cnt, arr) = freshen_exp m m_old cnt arr
      in
        (cnt, ArrLen arr)) ∧
-  freshen_exp m cnt (ArrSel arr idx) =
+  freshen_exp m m_old cnt (ArrSel arr idx) =
     (let
-       (cnt, arr) = freshen_exp m cnt arr;
-       (cnt, idx) = freshen_exp m cnt idx
+       (cnt, arr) = freshen_exp m m_old cnt arr;
+       (cnt, idx) = freshen_exp m m_old cnt idx
      in
        (cnt, ArrSel arr idx)) ∧
-  freshen_exp m cnt (FunCall n args) =
+  freshen_exp m m_old cnt (FunCall n args) =
     (let
-       (cnt, args) = freshen_exps m cnt args
+       (cnt, args) = freshen_exps m m_old cnt args
      in
        (cnt, FunCall n args)) ∧
-  freshen_exp m cnt (Forall (old, vt) e) =
+  freshen_exp m m_old cnt (Forall (old, vt) e) =
     (let
        (cnt, m) = add_fresh m cnt old;
-       (cnt, e) = freshen_exp m cnt e
+       (cnt, e) = freshen_exp m m_old cnt e
      in
        (cnt, Forall (lookup m old, vt) e)) ∧
-  freshen_exps m cnt [] = (cnt, []) ∧
-  freshen_exps m cnt (e::es) =
+  freshen_exp m m_old cnt (Old e) =
+    (let (cnt, e) = freshen_exp m_old m_old cnt e in (cnt, Old e)) ∧
+  freshen_exps m m_old cnt [] = (cnt, []) ∧
+  freshen_exps m m_old cnt (e::es) =
     (let
-       (cnt, e) = freshen_exp m cnt e;
-       (cnt, es) = freshen_exps m cnt es
+       (cnt, e) = freshen_exp m m_old cnt e;
+       (cnt, es) = freshen_exps m m_old cnt es
      in
        (cnt, (e::es)))
 Termination
   wf_rel_tac ‘measure $ λx. case x of
-                            | INL (_,_,e) => exp_size e
-                            | INR (_,_,e) => list_size exp_size e’
+                            | INL (_,_,_,e) => exp_size e
+                            | INR (_,_,_,e) => list_size exp_size e’
 End
 
 Definition freshen_lhs_exp_def:
-  (freshen_lhs_exp m cnt (VarLhs old) =
+  (freshen_lhs_exp m m_old cnt (VarLhs old) =
      (cnt, VarLhs (lookup m old))) ∧
-  freshen_lhs_exp m cnt (ArrSelLhs arr idx) =
-  let (cnt, arr) = freshen_exp m cnt arr in
-  let (cnt, idx) = freshen_exp m cnt idx in
+  freshen_lhs_exp m m_old cnt (ArrSelLhs arr idx) =
+  let (cnt, arr) = freshen_exp m m_old cnt arr in
+  let (cnt, idx) = freshen_exp m m_old cnt idx in
     (cnt, ArrSelLhs arr idx)
 End
 
 Definition freshen_lhs_exps_def:
-  (freshen_lhs_exps m cnt [] = (cnt, [])) ∧
-  freshen_lhs_exps m cnt (le::les) =
-  let (cnt, le) = freshen_lhs_exp m cnt le in
-  let (cnt, les) = freshen_lhs_exps m cnt les in
+  (freshen_lhs_exps m m_old cnt [] = (cnt, [])) ∧
+  freshen_lhs_exps m m_old cnt (le::les) =
+  let (cnt, le) = freshen_lhs_exp m m_old cnt le in
+  let (cnt, les) = freshen_lhs_exps m m_old cnt les in
     (cnt, le::les)
 End
 
 Definition freshen_rhs_exp_def:
-  (freshen_rhs_exp m cnt (ExpRhs e) =
-   let (cnt, e) = freshen_exp m cnt e in
+  (freshen_rhs_exp m m_old cnt (ExpRhs e) =
+   let (cnt, e) = freshen_exp m m_old cnt e in
      (cnt, ExpRhs e)) ∧
-  freshen_rhs_exp m cnt (ArrAlloc len init_v) =
-  let (cnt, len) = freshen_exp m cnt len in
-  let (cnt, init_v) = freshen_exp m cnt init_v in
+  freshen_rhs_exp m m_old cnt (ArrAlloc len init_v) =
+  let (cnt, len) = freshen_exp m m_old cnt len in
+  let (cnt, init_v) = freshen_exp m m_old cnt init_v in
     (cnt, ArrAlloc len init_v)
 End
 
 Definition freshen_rhs_exps_def:
-  (freshen_rhs_exps m cnt [] = (cnt, [])) ∧
-  freshen_rhs_exps m cnt (re::res) =
-  let (cnt, re) = freshen_rhs_exp m cnt re in
-  let (cnt, res) = freshen_rhs_exps m cnt res in
+  (freshen_rhs_exps m m_old cnt [] = (cnt, [])) ∧
+  freshen_rhs_exps m m_old cnt (re::res) =
+  let (cnt, re) = freshen_rhs_exp m m_old cnt re in
+  let (cnt, res) = freshen_rhs_exps m m_old cnt res in
     (cnt, re::res)
 End
 
 Definition freshen_stmt_def:
-  (freshen_stmt m cnt Skip = (cnt, Skip)) ∧
-  (freshen_stmt m cnt (Assert tst) =
-   let (cnt, tst) = freshen_exp m cnt tst in
+  (freshen_stmt m m_old cnt Skip = (cnt, Skip)) ∧
+  (freshen_stmt m m_old cnt (Assert tst) =
+   let (cnt, tst) = freshen_exp m m_old cnt tst in
      (cnt, Assert tst)) ∧
-  (freshen_stmt m cnt (Then stmt₀ stmt₁) =
-   let (cnt, stmt₀) = freshen_stmt m cnt stmt₀ in
-   let (cnt, stmt₁) = freshen_stmt m cnt stmt₁ in
+  (freshen_stmt m m_old cnt (Then stmt₀ stmt₁) =
+   let (cnt, stmt₀) = freshen_stmt m m_old cnt stmt₀ in
+   let (cnt, stmt₁) = freshen_stmt m m_old cnt stmt₁ in
      (cnt, Then stmt₀ stmt₁)) ∧
-  (freshen_stmt m cnt (If tst thn els) =
-   let (cnt, tst) = freshen_exp m cnt tst in
-   let (cnt, thn) = freshen_stmt m cnt thn in
-   let (cnt, els) = freshen_stmt m cnt els in
+  (freshen_stmt m m_old cnt (If tst thn els) =
+   let (cnt, tst) = freshen_exp m m_old cnt tst in
+   let (cnt, thn) = freshen_stmt m m_old cnt thn in
+   let (cnt, els) = freshen_stmt m m_old cnt els in
      (cnt, If tst thn els)) ∧
-  (freshen_stmt m cnt (Dec local scope) =
+  (freshen_stmt m m_old cnt (Dec local scope) =
    let (old, vt) = local in
    let (cnt, m) = add_fresh m cnt old in
-   let (cnt, scope) = freshen_stmt m cnt scope in
+   let (cnt, scope) = freshen_stmt m m_old cnt scope in
      (cnt, Dec (lookup m old, vt) scope)) ∧
-  (freshen_stmt m cnt (Assign ass) =
-   let (cnt, rhss) = freshen_rhs_exps m cnt (MAP SND ass) in
-   let (cnt, lhss) = freshen_lhs_exps m cnt (MAP FST ass) in
+  (freshen_stmt m m_old cnt (Assign ass) =
+   let (cnt, rhss) = freshen_rhs_exps m m_old cnt (MAP SND ass) in
+   let (cnt, lhss) = freshen_lhs_exps m m_old cnt (MAP FST ass) in
      (cnt, Assign (ZIP (lhss, rhss)))) ∧
-  (freshen_stmt m cnt (While grd invs decrs mods body) =
-   let (cnt, grd) = freshen_exp m cnt grd in
-   let (cnt, invs) = freshen_exps m cnt invs in
-   let (cnt, decrs) = freshen_exps m cnt decrs in
-   let (cnt, mods) = freshen_exps m cnt mods in
-   let (cnt, body) = freshen_stmt m cnt body in
+  (freshen_stmt m m_old cnt (While grd invs decrs mods body) =
+   let (cnt, grd) = freshen_exp m m_old cnt grd in
+   let (cnt, invs) = freshen_exps m m_old cnt invs in
+   let (cnt, decrs) = freshen_exps m m_old cnt decrs in
+   let (cnt, mods) = freshen_exps m m_old cnt mods in
+   let (cnt, body) = freshen_stmt m m_old cnt body in
      (cnt, While grd invs decrs mods body)) ∧
-  (freshen_stmt m cnt (Print e ty) =
-   let (cnt, e) = freshen_exp m cnt e in
+  (freshen_stmt m m_old cnt (Print e ty) =
+   let (cnt, e) = freshen_exp m m_old cnt e in
      (cnt, Print e ty)) ∧
-  (freshen_stmt m cnt (MetCall lhss n args) =
-   let (cnt, args) = freshen_exps m cnt args in
-   let (cnt, lhss) = freshen_lhs_exps m cnt lhss in
+  (freshen_stmt m m_old cnt (MetCall lhss n args) =
+   let (cnt, args) = freshen_exps m m_old cnt args in
+   let (cnt, lhss) = freshen_lhs_exps m m_old cnt lhss in
      (cnt, MetCall lhss n args)) ∧
-  freshen_stmt m cnt Return = (cnt, Return)
+  freshen_stmt m m_old cnt Return = (cnt, Return)
 End
 
 Definition map_add_fresh_def:
@@ -161,22 +163,22 @@ Definition freshen_member_def:
    let (out_ns, out_ts) = UNZIP outs in
    let (cnt, m) = map_add_fresh m cnt out_ns in
    let out_ns = MAP (lookup m) out_ns in
-   let (cnt, reqs) = freshen_exps m cnt reqs in
-   let (cnt, ens) = freshen_exps m cnt ens in
-   let (cnt, reads) = freshen_exps m cnt reads in
-   let (cnt, decrs) = freshen_exps m cnt decrs in
-   let (cnt, mods) = freshen_exps m cnt mods in
-   let (cnt, body) = freshen_stmt m cnt body in
+   let (cnt, reqs) = freshen_exps m m cnt reqs in
+   let (cnt, ens) = freshen_exps m m cnt ens in
+   let (cnt, reads) = freshen_exps m m cnt reads in
+   let (cnt, decrs) = freshen_exps m m cnt decrs in
+   let (cnt, mods) = freshen_exps m m cnt mods in
+   let (cnt, body) = freshen_stmt m m cnt body in
      Method name (ZIP (in_ns, in_ts)) reqs ens reads
             decrs (ZIP (out_ns, out_ts)) mods body) ∧
   freshen_member (Function name ins res_t reqs reads decrs body) =
   (let (in_ns, in_ts) = UNZIP ins in
    let (cnt, m) = map_add_fresh [] 0 in_ns in
    let in_ns = MAP (lookup m) in_ns in
-   let (cnt, reqs) = freshen_exps m cnt reqs in
-   let (cnt, reads) = freshen_exps m cnt reads in
-   let (cnt, decrs) = freshen_exps m cnt decrs in
-   let (cnt, body) = freshen_exp m cnt body in
+   let (cnt, reqs) = freshen_exps m m cnt reqs in
+   let (cnt, reads) = freshen_exps m m cnt reads in
+   let (cnt, decrs) = freshen_exps m m cnt decrs in
+   let (cnt, body) = freshen_exp m m cnt body in
      Function name (ZIP (in_ns, in_ts)) res_t reqs reads decrs body)
 End
 
